code/ecdsap256/Hacl.Impl.P256.Qinv.fsti
@@ -8,26 +8,26 @@ module ST = FStar.HyperStack.ST
 open Lib.IntTypes
 open Lib.Buffer
 
-open Spec.ECDSA
 open Hacl.Spec.P256.Felem
-open Hacl.Impl.P256.Bignum
 open Hacl.Impl.P256.Scalar
 
 module S = Spec.P256
+module SD = Spec.ECDSA
 
-#reset-options " --z3rlimit 200"
+#set-options "--z3rlimit 30 --fuel 0 --ifuel 0"
 
-// qinv
-val montgomery_ladder_exponent: a:felem -> Stack unit
+// TODO: pass a resulting array
+val qinv: a:felem -> Stack unit
   (requires fun h -> live h a /\ as_nat h a < S.order)
   (ensures fun h0 _ h1 -> modifies (loc a) h0 h1 /\
-    fromDomain_ (as_nat h1 a) == exponent_spec (fromDomain_ (as_nat h0 a)) /\
-    as_nat h1 a < S.order)
+    as_nat h1 a < S.order /\
+    qmont_as_nat h1 a == S.qinv (qmont_as_nat h0 a))
 
+// TODO: rm
 val multPowerPartial: s:felem -> a:felem -> b:felem -> result:felem -> Stack unit
   (requires fun h ->
     live h a /\ live h b /\ live h result /\
     as_nat h a < S.order /\ as_nat h b < S.order /\
-    fromDomain_ (as_nat h a) == exponent_spec (fromDomain_ (fromDomain_ (as_nat h s))))
+    fromDomain_ (as_nat h a) == SD.exponent_spec (fromDomain_ (fromDomain_ (as_nat h s))))
   (ensures fun h0 _ h1 -> modifies (loc result) h0 h1 /\
     as_nat h1 result = (S.pow (as_nat h0 s) (S.order - 2) * (as_nat h0 b)) % S.order)
